Comparison proofs.

rocq-bluerock-brick/theories/lang/cpp/syntax/extras.v
@@ -1,5 +1,5 @@
 (*
- * Copyright (c) 2024 BlueRock Security, Inc.
+ * Copyright (c) 2024-2025 BlueRock Security, Inc.
  * This software is distributed under the terms of the BedRock Open-Source License.
  * See the LICENSE-BedRock file in the repository root for details.
  *)
@@ -13,14 +13,23 @@ Proof.
   constructor; intros *; apply numbers.positive_comparison.
 Qed.
 
+Definition by_prim_tag_comparison {T} (f : T -> _)
+  : Comparison (fun a b => PrimInt63.compare (f a) (f b)).
+Proof. constructor; intros *; [ apply PString.char63_compare_antisym | eapply PString.char63_compare_trans ]. Qed.
+
+Lemma by_prim_tag_leibniz : ∀ {T : Type} (f : T → _),
+    (forall x y, match PrimInt63.compare (f x) (f y) with
+            | Eq => x = y
+            | _ => True
+            end) →
+    LeibnizComparison (λ a b : T, PrimInt63.compare (f a) (f b)).
+Proof. intros. red. intros. specialize (H a b). rewrite H0 in H. done. Qed.
+
 #[global] Instance function_qualifiers_comparison : Comparison function_qualifiers.compare.
-Proof. (* eapply by_tag_comparison. Qed. *) Admitted.
+Proof. apply by_prim_tag_comparison. Qed.
 
 #[global] Instance function_qualifiers_leibniz_cmp : LeibnizComparison function_qualifiers.compare.
-Proof.
-(*  apply by_tag_leibniz.
-  compute. destruct x, y; congruence.
-Qed. *) Admitted.
+Proof. apply by_prim_tag_leibniz. compute. by destruct x, y; compute. Qed.
 
 #[global] Instance function_quailfiers_eq_dec : EqDecision function_qualifiers.t :=
   from_comparison.
